Java/src/Semantics/SemCmd.v
@@ -1,6 +1,6 @@
 Require Import Program SepAlg OpenILogic AssertionLogic SpecLogic SepAlgMap.
-Require Import MapInterface MapFacts.
-Require Import ILInsts ILogic ILEmbed Open Subst Stack Lang.
+Require Import MapInterface MapFacts Omega.
+Require Import ILInsts ILogic ILEmbed Open Stack Lang Subst.
 
 Import SepAlgNotations.
 
